src/Language/PlutusIR/Semantics/Dynamic/Deterministic.v
@@ -1,0 +1,268 @@
+Require Import PlutusCert.Language.PlutusIR.
+Import NamedTerm.
+Require Import PlutusCert.Language.PlutusIR.Semantics.Dynamic.
+
+(** * [substitute] is deterministic*)
+
+Definition P_substitute (x : name) (s t t' : Term) : Prop :=
+  forall t'',
+    substitute x s t t'' ->
+    t' = t''. 
+
+Definition P_substitute_bindings_nonrec (x : name) (s : Term) (bs bs' : list Binding) : Prop :=
+  forall bs'',
+    substitute_bindings_nonrec x s bs bs'' ->
+    bs' = bs''.
+
+Definition P_substitute_bindings_rec (x : name) (s : Term) (bs bs' : list Binding) : Prop :=
+  forall bs'',
+    substitute_bindings_rec x s bs bs'' ->
+    bs' = bs''.
+        
+Definition P_substitute_binding (x : name) (s : Term) (b b' : Binding) : Prop :=
+  forall b'',
+    substitute_binding x s b b'' ->
+    b' = b''.
+
+Theorem substitute__deterministic : 
+  (forall x s t t', substitute x s t t' -> P_substitute x s t t') /\
+  (forall x s bs bs', substitute_bindings_nonrec x s bs bs' -> P_substitute_bindings_nonrec x s bs bs') /\
+  (forall x s bs bs', substitute_bindings_rec x s bs bs' -> P_substitute_bindings_rec x s bs bs') /\
+  (forall x s b b', substitute_binding x s b b' -> P_substitute_binding x s b b').
+Proof.
+  apply substitute__mutind with 
+    (P := P_substitute)
+    (P0 := P_substitute_bindings_nonrec)
+    (P1 := P_substitute_bindings_rec)
+    (P2 := P_substitute_binding). 
+Admitted. (* TODO *)
+
+(** * [eval] is deterministic *)
+
+Theorem eval_defaultfun__deterministic : forall t v1 v2,
+  eval_defaultfun t v1 ->
+  eval_defaultfun t v2 ->
+  v1 = v2.
+Proof. Admitted. (* TODO *)
+
+Definition P_eval x y1 :=
+  forall y2,
+    x ==> y2 ->
+    y1 = y2.
+
+Definition P_eval_bindings_non_rec x y1 :=
+  forall y2,
+    eval_bindings_nonrec x y1 ->
+    eval_bindings_nonrec x y2 ->
+    y1 = y2.
+
+Theorem eval__deterministic : forall x y1,
+  x ==> y1 ->
+  P_eval x y1.
+Proof.
+  apply eval__ind with (P := P_eval) (P0 := P_eval_bindings_non_rec).
+  - (* E_Let *)
+    intros. unfold P_eval. intros.
+    inversion H1. subst.
+    apply H0.
+    + assumption.
+    + assumption.
+  - (* E_LetRec *)
+    intros. unfold P_eval. intros.
+    inversion H. subst.
+    reflexivity.
+  - (* E_TyAbs *)
+    intros. unfold P_eval. intros.
+    inversion H1. subst.
+    f_equal.
+    apply H0.
+    assumption.
+  - (* E_LamAbs *)
+    intros. unfold P_eval. intros.
+    inversion H. subst.
+    reflexivity.
+  - (* E_Apply *)
+    intros. unfold P_eval. intros.
+    inversion H6.
+    + (* E_Apply *)
+      subst.
+      apply H5.
+      assert (LamAbs x T t0 = LamAbs x0 T0 t5). {
+        apply H0. assumption.
+      }
+      inversion H7. subst.
+      assert (v2 = v1). {
+        apply H2. assumption.
+      }
+      subst.
+      assert (t0'0 = t0'). {
+        apply substitute__deterministic with x0 v1 t5.
+        + assumption.
+        + assumption.
+      }
+      subst. 
+      assumption.
+    + (* E_ApplyBuiltin1 *)
+      subst.
+      assert (LamAbs x T t0 = v1). {
+        apply H0. assumption.
+      }
+      subst.
+      inversion H13.
+    + (* E_ApplyBuiltin2 *) 
+      subst. 
+      assert (LamAbs x T t0 = v1). {
+        apply H0. assumption.
+      }
+      subst.
+      inversion H10.
+  - (* E_Constant *)
+    intros. unfold P_eval. intros.
+    inversion H. subst.
+    reflexivity.
+  - (* E_Builtin *)
+    intros. unfold P_eval. intros.
+    inversion H. subst.
+    reflexivity.
+  - (* E_ApplyBuiltin1 *)
+    intros. unfold P_eval. intros.
+    inversion H5.
+    + (* E_Apply *) 
+      subst.
+      assert (v1 = LamAbs x T t4). {
+        apply H0. assumption.
+      }
+      subst.
+      inversion H4.
+    + (* E_AppltBuiltin1 *)
+      subst.
+      assert (v1 = v0). {
+        apply H0. assumption.
+      }
+      subst.
+      assert (v2 = v3). {
+        apply H3. assumption.
+      }
+      subst.
+      reflexivity.
+    + (* E_ApplyBuiltin2 *)
+      subst.
+      assert (v1 = v0). {
+        apply H0. assumption.
+      }
+      subst.
+      assert (v2 = v3). {
+        apply H3. assumption.
+      }
+      subst.
+      apply H11 in H4.
+      destruct H4.
+  - (* E_ApplyBuiltin3 *)
+    intros. unfold P_eval. intros.
+    inversion H6. subst.
+    + (* E_Apply *) 
+      subst.
+      assert (v1 = LamAbs x T t4). {
+        apply H0. assumption.
+      }
+      subst.
+      inversion H1.
+    + (* E_ApplyBuiltin1 *)
+      subst.
+      assert (v1 = v3). {
+        apply H0. assumption.
+      }
+      subst.
+      assert (v2 = v4). {
+        apply H3. assumption.
+      }
+      subst.
+      apply H4 in H13.
+      destruct H13.
+    + (* E_ApplyBuiltin2 *)
+      subst.
+      assert (v1 = v3). {
+        apply H0. assumption.
+      }
+      subst.
+      assert (v2 = v4). {
+        apply H3. assumption.
+      }
+      subst.
+      apply eval_defaultfun__deterministic with (Apply v3 v4).
+      * assumption.
+      * assumption.
+  - (* E_TyInstBuiltin1 *)
+    intros. unfold P_eval. intros.
+    inversion H1.
+    + (* E_TyInstBuiltin1 *)
+      reflexivity.
+    + (* E_TyInst *)  
+      subst.
+      assert (Builtin IfThenElse = TyAbs X K y2). {
+        apply H0. assumption.
+      }
+      inversion H2.
+  - (* E_TyInst *)
+    intros. unfold P_eval. intros.
+    inversion H1.
+    + (* E_TyInstBuiltin1 *)
+      subst.
+      assert (TyAbs X K v0 = Builtin IfThenElse). {
+        apply H0. assumption.
+      }
+      inversion H2.
+    + (* E_TyInst *)
+      subst.
+      assert (TyAbs X K v0 = TyAbs X0 K0 y2). {
+        apply H0. assumption.
+      }
+      inversion H2. subst.
+      reflexivity.
+  - (* E_Error *)
+    intros. unfold P_eval. intros.
+    inversion H. subst.
+    reflexivity.
+  - (* E_IWrap *)
+    intros. unfold P_eval. intros.
+    inversion H1. subst.
+    f_equal.
+    apply H0.
+    assumption.
+  - (* E_Unwrap *)
+    intros. unfold P_eval. intros.
+    inversion H1. subst.
+    assert (IWrap F T v0 = IWrap F0 T0 y2). {
+      apply H0. assumption.  
+    }
+    inversion H2. subst.
+    reflexivity.
+  
+  - (* E_NilB_NonRec  *)
+    intros. unfold P_eval_bindings_non_rec. intros.
+    inversion H1. subst.
+    inversion H2. subst.
+    apply H0. assumption.
+  - (* E_ConsB_NonRec *)
+    intros. unfold P_eval_bindings_non_rec. intros.
+    inversion H6. subst.
+    assert (vb = vb0). {
+      apply H0. assumption.
+    }
+    subst.
+    assert (t' = t'0). {
+      apply substitute__deterministic in H2.
+      apply H2 in H16.
+      assumption.
+    }
+    subst.
+    assert (bs' = bs'0). {
+      apply substitute__deterministic in H1.
+      apply H1 in H15.
+      assumption.
+    }
+    subst.
+    apply H4.
+    + assumption.
+    + assumption.
+Qed.
