src/Language/PlutusIR/Semantics/TypeSafety/Preservation.v
@@ -1,0 +1,173 @@
+Require Import PlutusCert.Language.PlutusIR.
+Import NamedTerm.
+Require Import PlutusCert.Language.PlutusIR.Semantics.Static.
+Require Import PlutusCert.Language.PlutusIR.Semantics.Static.Implementations.Named.
+Require Import PlutusCert.Language.PlutusIR.Semantics.Dynamic.
+
+
+Lemma preservation__eval_defaultfun : forall ctx t T,
+    ctx |-+ t : T ->
+    forall v,
+      eval_defaultfun t v ->
+      ctx |-+ v : T.
+Proof. Admitted. (* TODO *)
+
+Theorem unique_kinds : forall ctx T K K',
+    ctx |-* T : K ->
+    ctx |-* T : K' ->
+    K = K'.
+Proof. Admitted.
+
+
+Definition P_term ctx t T := 
+  forall v, 
+    t ==> v -> 
+    ctx |-+ v : T.
+
+
+Definition P_constructor ctx c := ctx |-ok_c c.
+
+Definition P_bindings_nonrec ctx bs := 
+  forall t0 T v0,
+    ctx |-oks_nr bs ->    
+    P_term (append (flatten (List.map binds bs)) ctx) t0 T ->
+    eval_bindings_nonrec (Let NonRec bs t0) v0 ->
+    append (flatten (List.map binds bs)) ctx |-+ t0 : T ->
+    ctx |-+ v0 : T.
+
+Definition P_bindings_rec ctx bs := ctx |-oks_r bs.
+
+Definition P_binding ctx b := (*ctx |-ok b.*)
+  forall s x Tb tb vb t t' T,
+    b = TermBind s (VarDecl x Tb) tb ->
+    (binds (TermBind s (VarDecl x Tb) tb) ++ ctx) |-+ t : T ->
+    substitute x vb t t' ->
+    ctx |-+ t' : T.
+
+Axiom skip : forall P, P.
+
+Theorem preservation : forall (t : Term) (T : Ty),
+  empty |-+ t : T ->
+  P_term empty t T. 
+Proof.
+  intros.
+  eapply has_type__rect with (P := P_term) (P0 := P_constructor) (P1 := P_bindings_nonrec) (P2 := P_bindings_rec) (P3 := P_binding).
+  - intros. unfold P_term. intros.
+    inversion H6; subst.
+    unfold P_bindings_nonrec in H3.
+    eapply H3.
+    + apply H2.
+    + apply H5.
+    + apply H10.
+    + apply H4.
+  - apply skip. (* TODO *)
+  - (* T_Var *)
+    intros. unfold P_term. intros.
+    inversion H1. 
+  - (* T_TyAbs *)
+    intros. unfold P_term. intros.
+    inversion H2. subst.
+    apply T_TyAbs.
+    apply H1.
+    assumption.
+  - (* T_LamAbs *)
+    intros. unfold P_term. intros.
+    inversion H3. subst.
+    apply T_LamAbs.
+    + assumption.
+    + assumption.
+  - (* T_Apply *) 
+    intros. unfold P_term. intros.
+    inversion H4.
+    + subst. apply skip. (* TODO *)
+    + subst. 
+      apply T_Apply with T1.
+      * apply H1.
+        assumption.
+      * apply H3.
+        assumption.   
+    + subst.
+      apply preservation__eval_defaultfun with (Apply v1 v2).
+      * apply T_Apply with T1.
+        -- apply H1.
+           assumption.
+        -- apply H3.
+           assumption.
+      * assumption.
+  - (* T_Constant *)
+    intros. unfold P_term. intros.
+    inversion H0. subst.
+    apply T_Constant.
+  - (* T_Builtin *)
+    intros. unfold P_term. intros.
+    inversion H0. subst.
+    apply T_Builtin.
+  - (* T_TyInst *) 
+    intros. unfold P_term. intros.
+    inversion H4.
+    + subst.
+      apply T_TyInst with (T1 := T1) (X := X) (K2 := K2).
+      * apply H1.
+        assumption.
+      * assumption.
+      * assumption.
+    + subst. apply skip. (* TODO *)
+  - (* T_Error *)
+    intros. unfold P_term. intros.
+    inversion H1. subst.
+    apply T_Error.
+    assumption.
+  - (* T_IWrap *)
+    intros. unfold P_term. intros.
+    inversion H5. subst.
+    apply T_IWrap with (X := X) (K := K) (S := S).
+    + assumption.
+    + apply H2.
+      assumption.
+    + assumption.
+    + assumption.
+  - (* T_Unwrap *)
+    intros. unfold P_term. intros.
+    inversion H4. subst.
+    apply H1 in H6 as H7.
+    inversion H7. subst.
+    assert (K = K0) by eauto using unique_kinds.
+    subst. (* TODO: something with transitivity and free variables *)
+    apply skip.
+
+  - (* W_Con *)
+    intros. unfold P_constructor. 
+    apply W_Con.
+    assumption.
+
+  - intros. unfold P_bindings_nonrec. intros.
+    inversion H2. subst.
+    simpl in H3.
+    unfold P_term in H1.
+    simpl in H1.
+    apply H1.
+    apply H5.
+  - intros. unfold P_bindings_nonrec. unfold P_bindings_nonrec in H3. intros.
+      
+    inversion H6. subst.
+    eapply H1.
+    + reflexivity.
+    + simpl.
+      eapply H3.
+      * assumption.
+      * unfold flatten in H5.
+        unfold flatten in H5.
+        unfold append in H5.
+        simpl in H5. unfold extendT in H5. simpl in H5.
+        rewrite List.concat_app in H5. simpl in H5.
+        rewrite <- List.app_assoc in H5. simpl in H5.
+        apply H5.
+      * apply skip. 
+      * unfold flatten in H7.
+        unfold flatten in H7.
+        unfold append in H7.
+        simpl in H7. unfold extendT in H7. simpl in H7.
+        rewrite List.concat_app in H7. simpl in H7.
+        rewrite <- List.app_assoc in H7. simpl in H7.
+        apply H7.
+Abort.
